PlonkLean/Syntax.lean
@@ -2,18 +2,39 @@ import Lean
 import Lean.Elab.Term
 import PlonkLean.Semantics
 
--- TODO Just use Getter?
-def Expression s a := s → a
+structure ProcedureSignature where
+  params : List Type
+  ret    : Type
+
+def paramListToTuple (types : List Type) : Type := match types with
+  | [] => PUnit
+  | (x :: xs) => x × paramListToTuple xs
+
+-- structure Procedure' s (sig : ProcedureSignature) where
+  -- body : Stmt s
+  -- return_val : Getter sig.ret s
 
 /-- Syntactic program (with arbitrary Lean terms as expressions) -/
 inductive Stmt (s : Type) : Type 1 where
   | skip : Stmt s
-  | assign {a : Type} : Lens a s → Expression s a → Stmt s -- mutation
-  | sample {a : Type} : Lens a s → Expression s (SubProbability a) → Stmt s
-  | call {a : Type} : Lens a s → Expression s (Program s a) → Stmt s
+  | assign {a : Type} : Lens a s → Getter a s → Stmt s -- mutation
+  | sample {a : Type} : Lens a s → Getter (SubProbability a) s → Stmt s
+  | call' {sig : ProcedureSignature} :
+      -- We have to spell out all parts of the procedure, unfortunately
+      -- (Lean forbids the mutual induction with `Procedure`)
+      Lens sig.ret s → (paramListToTuple sig.params → Stmt s) → Getter sig.ret s
+        → Getter (paramListToTuple sig.params) s → Stmt s
   | seq : Stmt s → Stmt s → Stmt s                   -- c1; c2
-  | ifThenElse : (Expression s Bool) → Stmt s → Stmt s → Stmt s  -- if b then c1 else c2
-  | while : (Expression s Bool) → Stmt s → Stmt s           -- while b do c
+  | ifThenElse : (Getter Bool s) → Stmt s → Stmt s → Stmt s  -- if b then c1 else c2
+  | while : (Getter Bool s) → Stmt s → Stmt s           -- while b do c
+
+structure Procedure s (sig : ProcedureSignature) where
+  body : paramListToTuple sig.params → Stmt s
+  return_val : Getter sig.ret s
+
+def Stmt.call {sig} (x : Lens sig.ret s) (proc : Procedure s sig)
+      (params : Getter (paramListToTuple sig.params) s) : Stmt s :=
+  Stmt.call' x proc.body proc.return_val params
 
 /- # Syntax of programs -/
 
@@ -24,7 +45,7 @@ declare_syntax_cat ec_var
 syntax (name := ec_var_single) ident : ec_var
 syntax (name := ec_var_nary) "( " ident (", " ident)* " )" : ec_var
 syntax ec_var " <- " term ";" : ec_stmt
-syntax ec_var " <@ " term ";" : ec_stmt
+syntax ec_var " <@ " "[" term "]" term ";" : ec_stmt  -- TODO: Funny syntax! Fix!
 syntax ec_var " <$ " term ";" : ec_stmt
 syntax "{" ec_stmt* "}" : ec_stmt
 syntax "if" "(" term ")" ec_stmt ( "else" ec_stmt )? : ec_stmt
@@ -57,7 +78,7 @@ macro_rules
   | `([expr| $t:term]) => fixExpression t
   | `([ec| $x:ec_var <- $e:term;]) => `(Stmt.assign [var| $x] [expr| $e])
   | `([ec| $x:ec_var <$ $e:term;]) => `(Stmt.sample [var| $x] [expr| $e])
-  | `([ec| $x:ec_var <@ $e:term;]) => `(Stmt.call [var| $x] [expr| $e])
+  | `([ec| $x:ec_var <@ [ $e:term ] $f:term;]) => `(Stmt.call [var| $x] [expr| $e] [expr| $f])
   | `([ec| if ($b) $t:ec_stmt else $e:ec_stmt]) =>
       `(Stmt.ifThenElse [expr| $b] [ec| $t] [ec| $e])
   | `([ec| if ($b) $t:ec_stmt]) =>
@@ -73,27 +94,38 @@ macro_rules
 noncomputable
 def denotation {s : Type} : Stmt s → Program s Unit
 | Stmt.skip => do return ()
-| Stmt.assign x e => do let st ← Program.get_state; let result := e st; Program.set x result
-| Stmt.sample x e => do let st ← Program.get_state; let result ← (e st).toProgram; Program.set x result
-| Stmt.call x e => do let st ← Program.get_state; let result ← e st; Program.set x result
-| Stmt.ifThenElse c t e => do let st ← Program.get_state; let result := c st; if result then denotation t else denotation e
-| Stmt.while c t => while_loop (do let st ← Program.get_state; return c st) (denotation t)
+| Stmt.assign x e => do let st ← Program.get_state; let result := e.get st; Program.set x result
+| Stmt.sample x e => do
+    let st ← Program.get_state
+    let result ← (e.get st).toProgram
+    Program.set x result
+| Stmt.call' x b r p => do
+    let params ← Program.get p
+    denotation (b params)
+    let result <- Program.get r
+    Program.set x result
+| Stmt.ifThenElse c t e => do
+    let st ← Program.get_state
+    let result := c.get st
+    if result then denotation t else denotation e
+| Stmt.while c t => while_loop (do let st ← Program.get_state; return c.get st) (denotation t)
 | Stmt.seq p q => do denotation p; denotation q
 
 /- # Experiments -/
 
-axiom state : Type
-axiom x : Lens Nat state
-axiom a : Lens Nat state
-axiom b : Lens Nat state
+-- axiom state : Type
+-- axiom x : Lens Nat state
+-- axiom a : Lens Nat state
+-- axiom b : Lens Nat state
+--
+-- def $a := 5
+--
+-- #check [expr| $a + 1]
 
-def $a := 5
+-- TODO fix
+-- noncomputable
+-- def example_program := [ec|
+-- if ($x==1) { a <- 1; b <- 2; } else {}
+-- ]
 
-#check [expr| $a + 1]
-
-noncomputable
-def example_program := [ec|
-if ($x==1) { a <- 1; b <- 2; } else {}
-]
-
-#print example_program
+-- #print example_program
